examples/uint63nat/prims.c
@@ -1,0 +1,34 @@
+#include "values.h"
+#include "glue.h"
+#include <stdio.h>
+
+typedef enum { O, S } nat;
+
+value uint63_from_nat(value n) {
+  value temp = n;
+  unsigned long long i = 0;
+
+  while (get_Coq_Init_Datatypes_nat_tag(temp) == S) {
+    i++;
+    temp = get_Coq_Init_Datatypes_S_args(temp)->Coq_Init_Datatypes_S_arg_0;
+  }
+  return (i << 1) + 1;
+}
+
+value uint63_to_nat(struct thread_info *tinfo, value t) {
+  value i = t >> 1;
+  value temp = make_Coq_Init_Datatypes_nat_O();
+  while (i) {
+    temp = alloc_make_Coq_Init_Datatypes_nat_S(tinfo, temp);
+    i--;
+  }
+  return temp;
+}
+
+value uint63_add(value x, value y) {
+  return (((x >> 1) + (y >> 1)) << 1) + 1;
+}
+
+value uint63_mul(value x, value y) {
+  return (((x >> 1) * (y >> 1)) << 1) + 1;
+}
