examples/uint63nat/prims.h
@@ -1,0 +1,10 @@
+#include <stdio.h>
+#include "glue.h"
+
+value uint63_from_nat(value z);
+
+value uint63_to_nat(struct thread_info *tinfo, value t);
+
+value uint63_add(value x, value y);
+
+value uint63_mul(value x, value y);
