library/modelled.v
@@ -14,6 +14,10 @@ Ltac eq_refl_match :=
   (* | [ _ : context[match ?x with | eq_refl => _ end] |- _] => destruct x *)
   end.
 
+Ltac prim_rewrites :=
+  repeat eq_refl_match;
+  rewrite ?from_to, ?to_from.
+
 Ltac props x :=
   let P := fresh in
   pose proof x as P;
@@ -32,18 +36,20 @@ Inductive annotated : Type :=
                     annotated
 | TRANSPARENT : forall (A : Type) `{Rep A}, (option (A -> annotated)) -> annotated.
 
+(* Theorem InGraph_any : forall {A : Type}, InGraph A. *)
+(* Proof. intros. constructor. intros. exact False. Defined. *)
 Theorem Rep_any : forall {A : Type}, Rep A. Admitted.
 
 Fixpoint to_prim_fn_type (r : annotated) : Type :=
   match r with
   | TYPEPARAM f => forall (A : Type), to_prim_fn_type (f A Rep_any)
-  | OPAQUE pt mt M o =>
-      match o with
+  | OPAQUE pt mt Iso k =>
+      match k with
       | None => pt
       | Some fp => forall (p : pt), to_prim_fn_type (fp p)
       end
-  | TRANSPARENT t R o =>
-      match o with
+  | TRANSPARENT t Rep_A k =>
+      match k with
       | None => t
       | Some f => forall (x : t), to_prim_fn_type (f x)
       end
@@ -52,13 +58,13 @@ Fixpoint to_prim_fn_type (r : annotated) : Type :=
 Fixpoint to_model_fn_type (r : annotated) : Type :=
   match r with
   | TYPEPARAM f => forall (A : Type), to_model_fn_type (f A Rep_any)
-  | OPAQUE pt mt M o =>
-      match o with
+  | OPAQUE pt mt Iso k =>
+      match k with
       | None => mt
-      | Some fp => forall (m : mt), to_model_fn_type (fp (@to pt mt M m))
+      | Some fp => forall (m : mt), to_model_fn_type (fp (@to pt mt Iso m))
       end
-  | TRANSPARENT t R o =>
-      match o with
+  | TRANSPARENT t Rep_A k =>
+      match k with
       | None => t
       | Some f => forall (x : t), to_model_fn_type (f x)
       end
@@ -70,6 +76,35 @@ Record extern_properties :=
   ; model_fn : to_model_fn_type type_desc
   ; c_name : string
   }.
+
+(*
+From Equations Require Import Equations Signature.
+
+Ltac rewrite_apply lem t :=
+  let m := fresh "m" in
+  pose (m := t);
+  rewrite lem in m;
+  apply m.
+
+Equations model_spec_aux
+          (a : annotated)
+          (pt : to_prim_fn_type a)
+          (mt : to_model_fn_type a) : Prop :=
+model_spec_aux (@TYPEPARAM f) pt mt :=
+  forall (A : Type), model_spec_aux (f A Rep_any) (pt A) (mt A) ;
+model_spec_aux (@OPAQUE prim_type model_type Iso (Some k)) pt mt :=
+  forall (x : prim_type),
+    model_spec_aux (k x) (pt x)
+      (mt (ltac: (rewrite_apply from_to (@from prim_type model_type Iso x)))) ;
+      (* (ltac: (rewrite_apply from_to (mt (@from prim_type model_type Iso x)))) ; *)
+model_spec_aux (@OPAQUE prim_type model_type Iso None) pt mt :=
+  pt = to mt ;
+model_spec_aux (@TRANSPARENT A Rep_A (Some k)) pt mt :=
+  forall (x : A), model_spec_aux (k x) (pt x) (mt x) ;
+model_spec_aux (@TRANSPARENT A Rep_A None) pt mt :=
+  pt = mt.
+Check from_to.
+*)
 
 Fixpoint model_spec_aux
          (a : annotated)
@@ -91,352 +126,4 @@ Defined.
 Definition model_spec (ep : extern_properties) : Prop :=
   model_spec_aux (type_desc ep) (prim_fn ep) (model_fn ep).
 
-Require Import VeriFFI.generator.all.
 
-Obligation Tactic := gen.
-MetaCoq Run (gen_for Z).
-MetaCoq Run (gen_for nat).
-MetaCoq Run (gen_for bool).
-
-Module IntVerification.
-
-Module Type UInt63.
-  Axiom t : Type.
-  Axiom from_Z : Z -> t.
-  Axiom to_Z : t -> Z.
-  Axiom add : t -> t -> t.
-  Axiom mul : t -> t -> t.
-End UInt63.
-
-(* Axiom VSU : Type. *)
-(* Axiom int63_vsu : VSU. *)
-(* Axiom lift : forall {A : Type}, A -> VSU -> string -> A. *)
-
-Module FM <: UInt63.
-  Definition t := {z : Z | 0 <= z < 2^63}%Z.
-  Definition from_Z (z : Z) : t.
-    exists (Z.modulo z (2^63)).
-    apply Z_mod_lt.
-    constructor.
-  Defined.
-
-  Definition to_Z (z : t) : Z := proj1_sig z.
-
-  Lemma mod63_ok:
-    forall z, (0 <= z mod (2^63) < 2^63)%Z.
-  Proof.
-    intro. apply Z.mod_pos_bound.
-    apply Z.pow_pos_nonneg; lia.
-   Qed.
-
-  Definition add (x y: t) : t :=
-  let '(exist xz x_pf) := x in
-  let '(exist yz y_pf) := y in
-  let z := ((xz + yz) mod (2^63))%Z in
-  exist _ z (mod63_ok _).
-
-  Definition mul (x y: t) : t :=
-  let '(exist xz x_pf) := x in
-  let '(exist yz y_pf) := y in
-  let z := ((xz * yz) mod (2^63))%Z in
-  exist _ z (mod63_ok _).
-
-End FM.
-
-Module C : UInt63.
-  Axiom t : Type.
-  Axiom from_Z : Z -> t.
-  Axiom to_Z : t -> Z.
-  Axiom add : t -> t -> t.
-  Axiom mul : t -> t -> t.
-End C.
-
-Module UInt63_Proofs.
-  Axiom Isomorphism_t : Isomorphism C.t FM.t.
-
-  Definition from_Z_ep : extern_properties :=
-    {| type_desc :=
-        @TRANSPARENT Z Rep_Z
-           (Some (fun z => @OPAQUE _ _ Isomorphism_t None))
-     ; prim_fn := C.from_Z
-     ; model_fn := FM.from_Z
-     ; c_name := "int63_from_Z"
-     |}.
-
-  Definition to_Z_ep : extern_properties :=
-    {| type_desc :=
-        @OPAQUE _ _ Isomorphism_t
-           (Some (fun z => @TRANSPARENT Z Rep_Z None))
-     ; prim_fn := C.to_Z
-     ; model_fn := FM.to_Z
-     ; c_name := "int63_to_Z"
-     |}.
-
-  Definition add_ep : extern_properties :=
-    {| type_desc :=
-          @OPAQUE _ _ Isomorphism_t
-            (Some (fun i =>
-              @OPAQUE _ _ Isomorphism_t
-                (Some (fun i => @OPAQUE _ _ Isomorphism_t None))))
-     ; prim_fn := C.add
-     ; model_fn := FM.add
-     ; c_name := "int63_add"
-     |}.
-
-  Definition mul_ep : extern_properties :=
-    {| type_desc :=
-          @OPAQUE _ _ Isomorphism_t
-            (Some (fun i =>
-              @OPAQUE _ _ Isomorphism_t
-                (Some (fun i => @OPAQUE _ _ Isomorphism_t None))))
-     ; prim_fn := C.mul
-     ; model_fn := FM.mul
-     ; c_name := "int63_mul"
-     |}.
-
-  Axiom from_Z_properties : model_spec from_Z_ep.
-  Axiom to_Z_properties : model_spec to_Z_ep.
-  Axiom add_properties : model_spec add_ep.
-  Axiom mul_properties : model_spec mul_ep.
-
-  Lemma seven : C.to_Z (C.add (C.from_Z 3%Z) (C.from_Z 4%Z)) = 7%Z.
-  Proof.
-    props from_Z_properties.
-    props to_Z_properties.
-    props add_properties.
-    repeat eq_refl_match.
-    rewrite !from_to, !to_from.
-    unfold FM.to_Z, FM.add, FM.from_Z.
-    simpl.
-    rewrite Z.mod_small.
-    auto.
-    lia.
-  Qed.
-
-  Lemma add_assoc : forall (x y z : Z),
-    C.to_Z (C.add (C.from_Z x) (C.add (C.from_Z y) (C.from_Z z))) =
-    C.to_Z (C.add (C.add (C.from_Z x) (C.from_Z y)) (C.from_Z z)).
-  Proof.
-    intros x y z.
-    props from_Z_properties.
-    props to_Z_properties.
-    props add_properties.
-    repeat eq_refl_match.
-    rewrite !from_to, !to_from.
-    unfold FM.add, FM.from_Z, FM.to_Z.
-    simpl.
-    rewrite <- !(Z.add_mod y z).
-    rewrite <- !(Z.add_mod x y).
-    rewrite <- !(Z.add_mod).
-    f_equal.
-    apply Z.add_assoc.
-    all: lia.
-  Qed.
-
-  Lemma mul_add_distr_l : forall (x y z : Z),
-    C.to_Z (C.mul (C.from_Z x) (C.add (C.from_Z y) (C.from_Z z))) =
-    C.to_Z (C.add (C.mul (C.from_Z x) (C.from_Z y)) (C.mul (C.from_Z x) (C.from_Z z))).
-  Proof.
-    intros x y z.
-    props from_Z_properties.
-    props to_Z_properties.
-    props add_properties.
-    props mul_properties.
-    repeat eq_refl_match.
-    rewrite !from_to, !to_from.
-    unfold FM.mul, FM.add, FM.from_Z, FM.to_Z.
-    simpl.
-    pose (y' := Z.modulo y (Z.pow_pos 2 63)); fold y'.
-    pose (z' := Z.modulo z (Z.pow_pos 2 63)); fold z'.
-    rewrite <- Zplus_mod.
-    rewrite <- Z.mul_add_distr_l.
-    rewrite Zmult_mod_idemp_r.
-    auto.
-  Qed.
-
-  Lemma mul_add_distr_r : forall (x y z : Z),
-    C.to_Z (C.mul (C.add (C.from_Z x) (C.from_Z y)) (C.from_Z z)) =
-    C.to_Z (C.add (C.mul (C.from_Z x) (C.from_Z z)) (C.mul (C.from_Z y) (C.from_Z z))).
-  Proof.
-    intros x y z.
-    props from_Z_properties.
-    props to_Z_properties.
-    props add_properties.
-    props mul_properties.
-    repeat eq_refl_match.
-    rewrite !from_to, !to_from.
-    unfold FM.mul, FM.add, FM.from_Z, FM.to_Z.
-    simpl.
-    pose (x' := Z.modulo y (Z.pow_pos 2 63)); fold x'.
-    pose (y' := Z.modulo y (Z.pow_pos 2 63)); fold y'.
-    pose (z' := Z.modulo z (Z.pow_pos 2 63)); fold z'.
-    rewrite <- Zplus_mod.
-    rewrite <- Z.mul_add_distr_r.
-    rewrite Zmult_mod_idemp_l.
-    auto.
-  Qed.
-
-End UInt63_Proofs.
-
-End IntVerification.
-
-Module ArrayVerification.
-
-Module Type ArraySetup.
-  Axiom t : Type.
-  Axiom len: nat.
-  Axiom init : t.
-End ArraySetup.
-
-Module Type Array (E : ArraySetup).
-  Axiom state : Type.
-  Definition M (A : Type) : Type := state -> A * state.
-  Axiom pure : forall {A}, A -> M A.
-  Axiom bind : forall {A B}, M A -> (A -> M B) -> M B.
-  Axiom runM : forall {A}, M A -> A.
-  Axiom set : nat -> E.t -> M unit.
-  Axiom get : nat -> M (option E.t).
-End Array.
-
-(* Look at canon.replace_nth, invariants.replace_nth, sepalg_list.replace for lemmas *)
-Module FM (E : ArraySetup) <: Array E.
-  Definition state := list E.t.
-  Definition M (A : Type) : Type := state -> A * state.
-  Definition pure {A} (a : A) : M A := fun s => (a, s).
-  Definition bind {A B} (m : M A) (f : A -> M B) : M B :=
-    fun s => f (fst (m s)) (snd (m s)).
-    (* fun s => let '(a, s') := m s in f a s'. *)
-  Definition runM {A} (m : M A) : A :=
-    fst (m (repeat E.init E.len)).
-
-  Definition set (index : nat) (elt : E.t) : M unit :=
-    fun s => (tt, canon.replace_nth index s elt).
-
-  Definition get (index : nat) : M (option E.t) :=
-    fun s => (nth_error s index, s).
-
-End FM.
-
-Module C (E : ArraySetup) : Array E.
-  Axiom state : Type.
-  Definition M (A : Type) : Type := state -> A * state.
-  Axiom pure : forall {A}, A -> M A.
-  Axiom bind : forall {A B}, M A -> (A -> M B) -> M B.
-  Axiom runM : forall {A}, M A -> A.
-  Axiom set : nat -> E.t -> M unit.
-  Axiom get : nat -> M (option E.t).
-End C.
-
-Module Array_Proofs.
-  Module E.
-    Definition t := bool.
-    Definition len := 5.
-    Definition init := false.
-  End E.
-  Module FM := FM E.
-  Module C := C E.
-
-  Definition Rep_t : Rep E.t := Rep_bool.
-
-  Axiom Isomorphism_state : Isomorphism C.state FM.state.
-
-  Definition Isomorphism_M
-             {A A' : Type} (I : Isomorphism A A')
-             : Isomorphism (C.M A) (FM.M A').
-  Proof.
-    eauto using Isomorphism_fn, Isomorphism_state, Isomorphism_pair.
-  Qed.
-
-  Definition pure_ep : extern_properties :=
-    {| type_desc :=
-        @TYPEPARAM (fun (A : Type) `{Rep_A : Rep A} =>
-          @TRANSPARENT A Rep_A (Some (fun arr =>
-            @OPAQUE (C.M A) (FM.M A) (Isomorphism_M _) None)))
-     ; prim_fn := @C.pure
-     ; model_fn := @FM.pure
-     ; c_name := "m_pure"
-     |}.
-
-  Definition bind_ep : extern_properties :=
-    {| type_desc :=
-        @TYPEPARAM (fun (A : Type) `{Rep_A : Rep A} =>
-          @TYPEPARAM (fun (B : Type) `{Rep_B : Rep B} =>
-            @OPAQUE (C.M A) (FM.M A) (Isomorphism_M _) (Some (fun m =>
-              @OPAQUE (A -> C.M B) (A -> FM.M B) (Isomorphism_fn _ (Isomorphism_M _)) (Some (fun f =>
-                @OPAQUE (C.M B) (FM.M B) (Isomorphism_M _) None))))))
-     ; prim_fn := @C.bind
-     ; model_fn := @FM.bind
-     ; c_name := "m_bind"
-     |}.
-
-  Definition runM_ep : extern_properties :=
-    {| type_desc :=
-        @TYPEPARAM (fun (A : Type) `{Rep_A : Rep A} =>
-          @OPAQUE (C.M A) (FM.M A) (Isomorphism_M _)
-                  (Some (fun f => @TRANSPARENT A Rep_A None)))
-     ; prim_fn := @C.runM
-     ; model_fn := @FM.runM
-     ; c_name := "m_runM"
-     |}.
-
-  Definition set_ep : extern_properties :=
-    {| type_desc :=
-        @TRANSPARENT nat Rep_nat (Some (fun n =>
-          @TRANSPARENT E.t Rep_t (Some (fun a =>
-            @OPAQUE (C.M unit) (FM.M unit) (Isomorphism_M _) None))))
-     ; prim_fn := @C.set
-     ; model_fn := @FM.set
-     ; c_name := "array_set"
-     |}.
-
-  Definition get_ep : extern_properties :=
-    {| type_desc :=
-        @TRANSPARENT nat Rep_nat (Some (fun n =>
-          @OPAQUE (C.M (option E.t)) (FM.M (option E.t)) (Isomorphism_M _) None))
-     ; prim_fn := @C.get
-     ; model_fn := @FM.get
-     ; c_name := "array_get"
-     |}.
-
-  Axiom pure_properties : model_spec pure_ep.
-  Axiom bind_properties : model_spec bind_ep.
-  Axiom runM_properties : model_spec runM_ep.
-  Axiom set_properties : model_spec set_ep.
-  Axiom get_properties : model_spec get_ep.
-
-  Ltac prim_rewrites :=
-    repeat eq_refl_match;
-    rewrite ?from_to, ?to_from.
-
-  Arguments from A B {_}.
-  Arguments to A B {_}.
-
-  Lemma set_get :
-    forall (n : nat) (bound : n < E.len) (to_set : E.t),
-      (C.runM (C.bind (C.set n to_set) (fun _ => C.get n)))
-        =
-      (C.runM (C.pure (Some to_set))).
-  Proof.
-    intros n bound to_set.
-
-    props runM_properties.
-    prim_rewrites.
-    unfold FM.runM.
-
-    props bind_properties.
-    props pure_properties.
-    unfold FM.bind, FM.pure.
-    prim_rewrites.
-
-    props set_properties.
-    props get_properties.
-    prim_rewrites.
-
-    eapply canon.nth_error_replace_nth.
-    apply nth_error_repeat.
-    auto.
-  Qed.
-
-End Array_Proofs.
-
-End ArrayVerification.
