verification/specs_general.v
@@ -5,98 +5,17 @@ Kathrin Stark, 2021.
 This file contains a general specification for the alloc function,
 using a representation of constructors.
 *)
+Require Import Coq.Lists.List.
+Import ListNotations.
+
+Require Import VST.floyd.proofauto.
+Require Import CertiGraph.CertiGC.GCGraph.
 
 From VeriFFI Require Export library.base_representation.
 From VeriFFI Require Export library.meta.
 From VeriFFI Require Export verification.graph_add.
 (* From VeriFFI Require Export verification.example.glue. *)
 From VeriFFI Require Export verification.specs_library.
-
-
-(** ** 1. Representable Type Class
-
-A type representable in a graph consists of:
-1. a type, X_type, which will be representable in the graph
-2. a function, X_in_graph, which defines the representation in a graph
-3. consistency conditions on X_in_graph, X_has_v and X_monotone, needed to actually get the later proof through:
-   a. X_has_v: Whenever a node represents an element of X_type, then this node is present in the graph.
-   b. X_monotone: Adding (compatible) nodes to a graph doesn't change whether an element of a type is present in the graph.
- *)
-
-(* Record representable_X  := *)
-(*   { X_type : Type; *)
-(*     X_in_graph : graph -> X_type -> rep_type -> Prop; *)
-(*     X_has_v : forall g n v, X_in_graph g n (repNode v) -> graph_has_v g v; *)
-(*     X_monotone : forall g to lb e n p, *)
-(*         add_node_compatible g (new_copied_v g to) e *)
-(*         -> graph_has_gen g to *)
-(*         -> X_in_graph g n p *)
-(*         -> X_in_graph (add_node g to lb e) n p *)
-(*     }. *)
-
-(* Existing Class representable_X. *)
-
-(** ** 2. Encoding constructors
-
-The code of a constructor which allows parameters, indices, dependent arguments
-tailored to what we need for the specification.
-The representation uses a weak HOAS representation.
-See the examples section for more detailed examples.
-
-ARG is not strictly necessary as it is an instance of DEPARG, but simplifies the later representation.
- *)
-
-(* Inductive constrCode := *)
-(* (* the type parameters in parametric polymorphism, isn't represented immediately in memory, *)
-(* but the possibility for representation is needed later, e.g., A in [list A] *)
-(*  *) *)
-(*  | TYPEPARAM  : (representable_X -> constrCode) -> constrCode *)
-(* (* Non-type parameters of a fixed type which isn't represented in memory, e.g., n in [n < m] *) *)
-(*  | PARAM  : forall X : Type, (X -> constrCode) -> constrCode *)
-(* (* index, represented in memory, e.g. the index of a vector *) *)
-(*  | INDEX  : forall (X_: representable_X), (X_type X_ -> constrCode) -> constrCode *)
-(*  (* non-dependent version of arguments, argument represented in memory, e.g. for X/list X of cons *) *)
-(*  | ARG : representable_X -> constrCode -> constrCode *)
-(*  (* dependent argument, represented in memory, e.g. in positive_nat_list *) *)
-(*  | DEPARG : forall (X_: representable_X), (X_type X_ -> constrCode) -> constrCode *)
-(* (* the end type, e.g., list X for cons : forall X, X -> list X -> **list X** *) *)
-(*  | RES  : representable_X -> constrCode. *)
-
-
-(** Representation of data needed for the argument part of an instance of a constrCodeuctor, e.g., in the with clause of a specification.
-This will be a dependent tuple. *)
-(* Fixpoint args (c : constrCode) : Type := *)
-(*     match c with *)
-(*     | TYPEPARAM f => {X_ : representable_X & args (f X_) } *)
-(*     | PARAM X f => {x : X & args (f x) } *)
-(*     | INDEX X_ f => {x : X_type X_ & args (f x)} *)
-(*     | ARG X_ arg => (X_type X_ * args arg)%type *)
-(*     | DEPARG X_ f => {x : X_type X_ & args (f x) } *)
-(*     | RES x => unit *)
-(* end. *)
-
-(* (* Instance of result type *) *)
-(* Fixpoint getRes (c: constrCode) (xs : args c) : representable_X := *)
-(*   match c as l return (args l -> representable_X) with *)
-(*   | TYPEPARAM f => fun H => let (X_, xs') := H in getRes (f X_) xs' *)
-(*   | PARAM X f => fun H => let (x, xs') := H in getRes (f x) xs' *)
-(*   | INDEX X_ f => fun H => let (x, xs') := H in getRes (f x) xs' *)
-(*   | ARG X_ arg => fun H => let (x, xs') := H in getRes arg xs' *)
-(*   | DEPARG X_ f => fun H  => let (x, xs') := H in getRes (f x) xs' *)
-(*   | RES x => fun _ => x *)
-(*   end xs. *)
-
-(* (** Full description of a constructor: *)
-(*    fitting identifier, the code for the constructor, *)
-(*    and the corresponding Coq function for the constructor. *)
-
-(*   This is what MetaCoq will have to generate. *)
-(*  *) *)
-(* Record constructor_description := *)
-(* { name : ident; *)
-(*   constr : constrCode; *)
-(*   coqConstr : forall (xs : args constr), X_type (getRes constr xs) *)
-(* }. *)
 
 (** ** 3. A General Specification *)
 
@@ -170,10 +89,35 @@ Notation "'WITH'  x1 : t1 , x2 : t2 , x3 : t3 , x4 : t4 , x5 : t5 , x6 : t6 , x7
               x10 at level 0,
              P at level 100, Q at level 100) : funspec_scope.
 
+
+Theorem Rep_any : forall {A : Type}, Rep A. Admitted.
+Print rep_type.
+Print in_graphs.
+Print nat.
+Definition count (r : reific Rep) : nat := 0.
+
+(*
+Definition alloc_make_nat_S : funspec :=
+  WITH gv : globals, g : graph, p : rep_type,
+       x: nat, roots : roots_t, sh : share,
+       ti : val, outlier : outlier_t, f_info : fun_info, t_info : GCGraph.thread_info
+  PRE  [[ [thread_info ; tulong] ]]
+     PROP (is_in_graph g x p ;
+           writable_share sh)
+     PARAMS (ti ; rep_type_val g p)
+     SEP (full_gc g t_info roots outlier ti sh)
+  POST [ tulong ]
+    EX (p' : rep_type) (g' : graph) (t_info' : GCGraph.thread_info),
+      PROP (is_in_graph g' (S x) p' ;
+            gc_graph_iso g roots g' roots)
+      RETURN  (rep_type_val g' p')
+      SEP (full_gc g' t_info' roots outlier ti sh).
+        *)
+
+(* move ps to the spec args somehow instead of WITH args *)
 Definition alloc_make_spec_general
            (c : constructor_description)
            (n : nat) : (* ident * *) funspec :=
-  (* DECLARE _w (* FIXME to actual C fn names somehow? *) *)
     WITH gv : globals, g : graph, ps : list rep_type,
          xs : args (ctor_reific c), roots : roots_t, sh : share,
          ti : val, outlier : outlier_t, f_info : fun_info, t_info : GCGraph.thread_info
@@ -184,7 +128,7 @@ Definition alloc_make_spec_general
        (PARAMSx (ti :: map (fun p => rep_type_val g p) ps)
        (GLOBALSx nil
        (SEPx (full_gc g t_info roots outlier ti sh :: nil))))
-    POST [ tptr tulong ]
+    POST [ tulong ]
       EX (p' : rep_type) (g' : graph) (t_info' : GCGraph.thread_info),
         PROP (let r := result (ctor_reific c) xs in
               @is_in_graph (projT1 r) (@in_graph (projT1 r) (projT2 r)) g' (ctor_real c xs) p' ;
@@ -196,37 +140,38 @@ Definition alloc_make_spec_general
 
 (** ** 4. Examples *)
 
-(* Require Import VeriFFI.generator.InGraph. *)
-(* Require Import VeriFFI.generator.Rep. *)
-(* Require Import VeriFFI.generator.Desc. *)
-(* Unset Strict Unquote Universe Mode. *)
+(*
+Require Import VeriFFI.generator.InGraph.
+Require Import VeriFFI.generator.Rep.
+Require Import VeriFFI.generator.Desc.
+Unset Strict Unquote Universe Mode.
 
-(* (** *** 4.0 Non-dependent, no indices/parameters - nat *) *)
-(* Set Printing All. *)
-(* Set Printing Universes. *)
-(* MetaCoq Run (in_graph_gen list). *)
-(* MetaCoq Run (in_graph_gen nat). *)
-(* Instance Rep_nat : Rep nat. rep_gen. Defined. *)
-(* MetaCoq Run (desc_gen O). *)
-(* MetaCoq Run (desc_gen S). *)
+(** *** 4.0 Non-dependent, no indices/parameters - nat *)
+Set Printing All.
+Set Printing Universes.
+MetaCoq Run (in_graph_gen list).
+MetaCoq Run (in_graph_gen nat).
+Instance Rep_nat : Rep nat. rep_gen. Defined.
+MetaCoq Run (desc_gen O).
+MetaCoq Run (desc_gen S).
 
-(* (** nat has to be representable *) *)
-(* Variable nat_has: forall (g : graph) (n : nat) (v : VType), nat_in_graph g n (repNode v) -> graph_has_v g v. *)
+(** nat has to be representable *)
+Variable nat_has: forall (g : graph) (n : nat) (v : VType), nat_in_graph g n (repNode v) -> graph_has_v g v.
 
-(* Variable nat_monotone:   forall (g : graph) (to : nat) (lb : raw_vertex_block) (e : list (EType * (VType * VType))) *)
-(*     (n : nat) (p : rep_type), *)
-(*   add_node_compatible g (new_copied_v g to) e -> *)
-(*   graph_has_gen g to -> nat_in_graph g n p -> nat_in_graph (add_node g to lb e) n p. *)
+Variable nat_monotone:   forall (g : graph) (to : nat) (lb : raw_vertex_block) (e : list (EType * (VType * VType)))
+    (n : nat) (p : rep_type),
+  add_node_compatible g (new_copied_v g to) e ->
+  graph_has_gen g to -> nat_in_graph g n p -> nat_in_graph (add_node g to lb e) n p.
 
-(* Definition nat_representable: representable_X := *)
-(* Build_representable_X nat nat_in_graph nat_has nat_monotone. *)
+Definition nat_representable: representable_X :=
+Build_representable_X nat nat_in_graph nat_has nat_monotone.
 
-(* (** Constructor code  *) *)
-(* Definition SucCode := *)
-(*   ARG nat_representable (RES nat_representable). *)
+(** Constructor code  *)
+Definition SucCode :=
+  ARG nat_representable (RES nat_representable).
 
 
-(** *** 4.1 Parameters - Lists, cons
+*** 4.1 Parameters - Lists, cons
 
 Specification we want:
 
@@ -250,85 +195,84 @@ DECLARE _alloc_make_Coq_Init_Datatypes_list_cons
          )
      RETURN  (rep_type_val g' p')
      SEP (full_gc g' t_info' roots outlier ti sh).
-*)
 
-(** 4.1.1 List has to be representable. *)
-(* Parameter list_has : *)
-(* forall X (g : graph) (n : list (X_type X)) (v : VType), *)
-(*    list_in_graph (X_in_graph X) g n (repNode v) -> graph_has_v g v. *)
+4.1.1 List has to be representable.
+Parameter list_has :
+forall X (g : graph) (n : list (X_type X)) (v : VType),
+   list_in_graph (X_in_graph X) g n (repNode v) -> graph_has_v g v.
 
-(* Parameter list_monotone : *)
-(* forall X (g : graph) (to : nat) (lb : raw_vertex_block) (e : list (EType * (VType * VType))) *)
-(*      (n : list (X_type X)) (p : rep_type), *)
-(*    add_node_compatible g (new_copied_v g to) e -> *)
-(*    graph_has_gen g to -> *)
-(*    list_in_graph (X_in_graph X) g n p -> list_in_graph (X_in_graph X) (add_node g to lb e) n p. *)
+Parameter list_monotone :
+forall X (g : graph) (to : nat) (lb : raw_vertex_block) (e : list (EType * (VType * VType)))
+     (n : list (X_type X)) (p : rep_type),
+   add_node_compatible g (new_copied_v g to) e ->
+   graph_has_gen g to ->
+   list_in_graph (X_in_graph X) g n p -> list_in_graph (X_in_graph X) (add_node g to lb e) n p.
 
-(* Definition list_representable_X (X : representable_X) : representable_X := *)
-(*   Build_representable_X (list (X_type X)) (list_in_graph (X_in_graph X)) (list_has X) (list_monotone X). *)
+Definition list_representable_X (X : representable_X) : representable_X :=
+  Build_representable_X (list (X_type X)) (list_in_graph (X_in_graph X)) (list_has X) (list_monotone X).
 
-(* (** Constructor code  *) *)
-(* Definition consCode := *)
-(*   TYPEPARAM (fun X => ARG X (ARG (list_representable_X X) (RES (list_representable_X X)))). *)
+(** Constructor code  *)
+Definition consCode :=
+  TYPEPARAM (fun X => ARG X (ARG (list_representable_X X) (RES (list_representable_X X)))).
 
-(* (** Constructor description *) *)
-(* Definition consDescr : constructor_description. *)
-(* Proof. *)
-(* refine (Build_constructor_description _alloc_make_Coq_Init_Datatypes_list_cons consCode _). *)
-(* simpl. intros (X&x&xs&_). simpl. exact (x :: xs). *)
-(* Defined. *)
+(** Constructor description *)
+Definition consDescr : constructor_description.
+Proof.
+refine (Build_constructor_description _alloc_make_Coq_Init_Datatypes_list_cons consCode _).
+simpl. intros (X&x&xs&_). simpl. exact (x :: xs).
+Defined.
 
-(* Definition nilCode := *)
-(*   TYPEPARAM (fun X => RES (list_representable_X X)). *)
+Definition nilCode :=
+  TYPEPARAM (fun X => RES (list_representable_X X)).
 
-(* Definition nilDescr : constructor_description. *)
-(* Proof. *)
-(* refine (Build_constructor_description _alloc_make_Coq_Init_Datatypes_list_cons nilCode _). *)
-(* simpl. intros (X&_). simpl. exact nil. *)
-(* Defined. *)
+Definition nilDescr : constructor_description.
+Proof.
+refine (Build_constructor_description _alloc_make_Coq_Init_Datatypes_list_cons nilCode _).
+simpl. intros (X&_). simpl. exact nil.
+Defined.
 
-(* MetaCoq Run (in_graph_gen list). *)
-(* Instance Rep_list : forall A, Rep A -> Rep (list A). rep_gen. Defined. *)
-(* MetaCoq Run (desc_gen nil). *)
-(* MetaCoq Run (desc_gen cons). *)
+MetaCoq Run (in_graph_gen list).
+Instance Rep_list : forall A, Rep A -> Rep (list A). rep_gen. Defined.
+MetaCoq Run (desc_gen nil).
+MetaCoq Run (desc_gen cons).
 
 
-(* Definition graph_X_var  (args : {graph_X_var : representable_X & (X_type graph_X_var (* x *) * list (X_type graph_X_var) (* xs *))%type })  := let (graph_X_var, args') := args in graph_X_var. *)
+Definition graph_X_var  (args : {graph_X_var : representable_X & (X_type graph_X_var (* x *) * list (X_type graph_X_var) (* xs *))%type })  := let (graph_X_var, args') := args in graph_X_var.
 
-(* Definition x (args : {graph_X_var : representable_X & (X_type graph_X_var (* x *) * list (X_type graph_X_var) (* xs *))%type }) : X_type (graph_X_var args). *)
-(* Proof. *)
-(*   destruct args, p. exact x0. *)
-(* Defined. *)
+Definition x (args : {graph_X_var : representable_X & (X_type graph_X_var (* x *) * list (X_type graph_X_var) (* xs *))%type }) : X_type (graph_X_var args).
+Proof.
+  destruct args, p. exact x0.
+Defined.
 
-(* Definition xs (args : {graph_X_var : representable_X & (X_type graph_X_var (* x *) * list (X_type graph_X_var) (* xs *))%type }) : list (X_type (graph_X_var args)). *)
-(* Proof. *)
-(*   destruct args, p. exact l. *)
-(* Defined. *)
+Definition xs (args : {graph_X_var : representable_X & (X_type graph_X_var (* x *) * list (X_type graph_X_var) (* xs *))%type }) : list (X_type (graph_X_var args)).
+Proof.
+  destruct args, p. exact l.
+Defined.
 
-(* Definition alloc_make_list_cons_spec : ident * funspec := *)
-(* DECLARE _alloc_make_Coq_Init_Datatypes_list_cons *)
-(*   WITH gv : globals, g : graph, p_x : rep_type, p_xs : rep_type, args : {graph_X_var : representable_X & (X_type graph_X_var (* x *) * list (X_type graph_X_var) (* xs *))%type },    roots : roots_t, sh : share, ti : val, outlier : outlier_t, f_info : fun_info, t_info : GCGraph.thread_info *)
-(*   PRE  [thread_info, tulong, tulong] *)
-(*        PROP (X_in_graph (graph_X_var args) g (x args) p_x; *)
-(*             list_in_graph (X_in_graph (graph_X_var args)) g (xs args) p_xs; *)
-(*              writable_share sh *)
-(*              ) *)
-(*        PARAMS (ti; *)
-(*               rep_type_val g p_x; *)
-(*               rep_type_val g p_xs) *)
-(*        GLOBALS () *)
-(*        SEP ( full_gc g t_info roots outlier ti sh ) *)
-(*   POST [ tptr tulong ] *)
-(*      EX (p' : rep_type) (g' : graph) (t_info' : GCGraph.thread_info), *)
-(*      PROP (list_in_graph (X_in_graph (graph_X_var args)) g' ((x args) :: (xs args)) p'; *)
-(*            gc_graph_iso g roots g' roots *)
-(*          ) *)
-(*      RETURN  (rep_type_val g' p') *)
-(*      SEP (full_gc g' t_info' roots outlier ti sh). *)
+Definition alloc_make_list_cons_spec : ident * funspec :=
+DECLARE _alloc_make_Coq_Init_Datatypes_list_cons
+  WITH gv : globals, g : graph, p_x : rep_type, p_xs : rep_type, args : {graph_X_var : representable_X & (X_type graph_X_var (* x *) * list (X_type graph_X_var) (* xs *))%type },    roots : roots_t, sh : share, ti : val, outlier : outlier_t, f_info : fun_info, t_info : GCGraph.thread_info
+  PRE  [thread_info, tulong, tulong]
+       PROP (X_in_graph (graph_X_var args) g (x args) p_x;
+            list_in_graph (X_in_graph (graph_X_var args)) g (xs args) p_xs;
+             writable_share sh
+             )
+       PARAMS (ti;
+              rep_type_val g p_x;
+              rep_type_val g p_xs)
+       GLOBALS ()
+       SEP ( full_gc g t_info roots outlier ti sh )
+  POST [ tptr tulong ]
+     EX (p' : rep_type) (g' : graph) (t_info' : GCGraph.thread_info),
+     PROP (list_in_graph (X_in_graph (graph_X_var args)) g' ((x args) :: (xs args)) p';
+           gc_graph_iso g roots g' roots
+         )
+     RETURN  (rep_type_val g' p')
+     SEP (full_gc g' t_info' roots outlier ti sh).
 
-(* (** Definitional equality will be hard because of unit/all ps would have to be in a list. *)
-(*  Probably, we'll want funspec_sub instead. *) *)
-(* (* Lemma cons_same_spec :  alloc_make_list_cons_spec = alloc_make_spec_general consDescr. *)
+(** Definitional equality will be hard because of unit/all ps would have to be in a list. *)
+(*  Probably, we'll want funspec_sub instead. *)
+(* Lemma cons_same_spec :  alloc_make_list_cons_spec = alloc_make_spec_general consDescr. *)
 (* Proof. *)
 (*   unfold alloc_make_spec_general. simpl. *)
 (* Admitted. *)
@@ -337,47 +281,47 @@ DECLARE _alloc_make_Coq_Init_Datatypes_list_cons
 (* Proof. *)
 (*   unfold funspec_sub. *)
 (*   simpl. intuition. *)
-(* Admitted. *) *)
+(* Admitted. *)
 
-(* (** *** 4.2 Indices/silent arguments - Vector, cons *) *)
+(** *** 4.2 Indices/silent arguments - Vector, cons *)
 
-(* Inductive vector (A : Type) : nat -> Type := *)
-(*    | vnil : vector A 0%nat *)
-(*    | vcons : A -> forall n : nat, vector A n -> vector A (S n). *)
+Inductive vector (A : Type) : nat -> Type :=
+   | vnil : vector A 0%nat
+   | vcons : A -> forall n : nat, vector A n -> vector A (S n).
 
-(* (** 4.1.2 Vectors have to be representable - all this will be generated automatically. *) *)
-(* Variable _alloc_make_Coq_Init_Datatypes_vector_cons : ident. *)
+(** 4.1.2 Vectors have to be representable - all this will be generated automatically. *)
+Variable _alloc_make_Coq_Init_Datatypes_vector_cons : ident.
 
-(* Variable vector_in_graph : forall X n, (graph -> X -> rep_type -> Prop) -> graph -> vector X n -> rep_type -> Prop. *)
+Variable vector_in_graph : forall X n, (graph -> X -> rep_type -> Prop) -> graph -> vector X n -> rep_type -> Prop.
 
-(* Variable vector_has :   forall X n (g : graph) (n0 : vector (X_type X) n) (v : VType), *)
-(*   vector_in_graph (X_type X) n (X_in_graph X) g n0 (repNode v) -> graph_has_v g v. *)
+Variable vector_has :   forall X n (g : graph) (n0 : vector (X_type X) n) (v : VType),
+  vector_in_graph (X_type X) n (X_in_graph X) g n0 (repNode v) -> graph_has_v g v.
 
-(* Variable vector_monotone : forall X n (g : graph) (to : nat) (lb : raw_vertex_block) (e : list (EType * (VType * VType))) *)
-(*    (n0 : vector (X_type X) n) (p : rep_type), *)
-(*  add_node_compatible g (new_copied_v g to) e -> *)
-(*  graph_has_gen g to -> *)
-(*  vector_in_graph (X_type X) n (X_in_graph X) g n0 p -> *)
-(*  vector_in_graph (X_type X) n (X_in_graph X) (add_node g to lb e) n0 p. *)
+Variable vector_monotone : forall X n (g : graph) (to : nat) (lb : raw_vertex_block) (e : list (EType * (VType * VType)))
+   (n0 : vector (X_type X) n) (p : rep_type),
+ add_node_compatible g (new_copied_v g to) e ->
+ graph_has_gen g to ->
+ vector_in_graph (X_type X) n (X_in_graph X) g n0 p ->
+ vector_in_graph (X_type X) n (X_in_graph X) (add_node g to lb e) n0 p.
 
-(* Definition vector_representable_X (X : representable_X) (n :nat) : representable_X. *)
-(* Proof. *)
-(*   refine (Build_representable_X (vector (X_type X) n) (vector_in_graph (X_type X) n (X_in_graph X)) _ _). *)
-(*   - apply vector_has. *)
-(*   - apply vector_monotone. *)
-(* Defined. *)
+Definition vector_representable_X (X : representable_X) (n :nat) : representable_X.
+Proof.
+  refine (Build_representable_X (vector (X_type X) n) (vector_in_graph (X_type X) n (X_in_graph X)) _ _).
+  - apply vector_has.
+  - apply vector_monotone.
+Defined.
 
-(* (** Constructor code *) *)
-(* Definition vectorConsCode := TYPEPARAM  (fun X => (ARG X (INDEX nat_representable (fun n => ARG (vector_representable_X X n) (RES (vector_representable_X X (S n))))))). *)
+(** Constructor code *)
+Definition vectorConsCode := TYPEPARAM  (fun X => (ARG X (INDEX nat_representable (fun n => ARG (vector_representable_X X n) (RES (vector_representable_X X (S n))))))).
 
-(* (** Constructor description *) *)
-(* Definition vectorConsDescr : constructor_description. *)
-(* Proof. *)
-(* refine (Build_constructor_description _alloc_make_Coq_Init_Datatypes_list_cons vectorConsCode _). *)
-(* simpl. intros (X&x&n&xs&_). simpl. exact (vcons _ x n xs). *)
-(* Defined. *)
+(** Constructor description *)
+Definition vectorConsDescr : constructor_description.
+Proof.
+refine (Build_constructor_description _alloc_make_Coq_Init_Datatypes_list_cons vectorConsCode _).
+simpl. intros (X&x&n&xs&_). simpl. exact (vcons _ x n xs).
+Defined.
 
-(* (** *** 4.3 Parameters and indices mixed -  param_and_index. *)
+(** *** 4.3 Parameters and indices mixed -  param_and_index. *)
 
 (* The specification we'd want modulo a/b/pf being packed in a sigma type: *)
 
@@ -400,53 +344,53 @@ DECLARE _alloc_make_Coq_Init_Datatypes_list_cons
 (*          ) *)
 (*      RETURN  (rep_type_val g' p') *)
 (*      SEP (full_gc g' t_info' roots outlier ti sh). *)
-(* *) *)
+(* *)
 
-(* Inductive param_and_index (a b : nat) : (a < b)%nat -> Type := *)
-(* | foo : forall (pf : (a < b)%nat), param_and_index a b pf. *)
+Inductive param_and_index (a b : nat) : (a < b)%nat -> Type :=
+| foo : forall (pf : (a < b)%nat), param_and_index a b pf.
 
-(* Variable le_in_graph : forall (a b : nat), graph -> (a < b)%nat -> rep_type -> Prop. *)
+Variable le_in_graph : forall (a b : nat), graph -> (a < b)%nat -> rep_type -> Prop.
 
-(* Parameter le_has :   forall a b (g : graph) (n : (a < b)%nat) (v : VType), *)
-(*   le_in_graph a b g n (repNode v) -> graph_has_v g v. *)
+Parameter le_has :   forall a b (g : graph) (n : (a < b)%nat) (v : VType),
+  le_in_graph a b g n (repNode v) -> graph_has_v g v.
 
-(* Parameter le_c :  forall a b (g : graph) (to : nat) (lb : raw_vertex_block) (e : list (EType * (VType * VType))) *)
-(*     (n : (a < b)%nat) (p : rep_type), *)
-(*   add_node_compatible g (new_copied_v g to) e -> *)
-(*   graph_has_gen g to -> le_in_graph a b g n p -> le_in_graph a b (add_node g to lb e) n p. *)
+Parameter le_c :  forall a b (g : graph) (to : nat) (lb : raw_vertex_block) (e : list (EType * (VType * VType)))
+    (n : (a < b)%nat) (p : rep_type),
+  add_node_compatible g (new_copied_v g to) e ->
+  graph_has_gen g to -> le_in_graph a b g n p -> le_in_graph a b (add_node g to lb e) n p.
 
-(* Definition le_representable (a b : nat) : representable_X. *)
-(* refine (Build_representable_X (a < b)%nat (le_in_graph a b) (le_has a b) (le_c a b)). *)
-(* Defined. *)
+Definition le_representable (a b : nat) : representable_X.
+refine (Build_representable_X (a < b)%nat (le_in_graph a b) (le_has a b) (le_c a b)).
+Defined.
 
-(* Variable param_and_index_in_graph : forall (a b : nat) (pf : (a < b)%nat), graph -> param_and_index a b pf -> rep_type -> Prop. *)
+Variable param_and_index_in_graph : forall (a b : nat) (pf : (a < b)%nat), graph -> param_and_index a b pf -> rep_type -> Prop.
 
-(* Variable param_and_index_has :   forall a b (lex : (a < b)%nat) (g : graph) (n : param_and_index a b lex) (v : VType), *)
-(*   param_and_index_in_graph a b lex g n (repNode v) -> graph_has_v g v. *)
+Variable param_and_index_has :   forall a b (lex : (a < b)%nat) (g : graph) (n : param_and_index a b lex) (v : VType),
+  param_and_index_in_graph a b lex g n (repNode v) -> graph_has_v g v.
 
-(* Variable param_and_index_monotone:  forall a b (lex : (a < b)%nat) (g : graph) (to : nat) (lb : raw_vertex_block) (e : list (EType * (VType * VType))) *)
-(*    (n : param_and_index a b lex) (p : rep_type), *)
-(*  add_node_compatible g (new_copied_v g to) e -> *)
-(*  graph_has_gen g to -> *)
-(*  param_and_index_in_graph a b lex g n p -> *)
-(*  param_and_index_in_graph a b lex (add_node g to lb e) n p. *)
+Variable param_and_index_monotone:  forall a b (lex : (a < b)%nat) (g : graph) (to : nat) (lb : raw_vertex_block) (e : list (EType * (VType * VType)))
+   (n : param_and_index a b lex) (p : rep_type),
+ add_node_compatible g (new_copied_v g to) e ->
+ graph_has_gen g to ->
+ param_and_index_in_graph a b lex g n p ->
+ param_and_index_in_graph a b lex (add_node g to lb e) n p.
 
-(* Definition param_and_index_representable : forall  (a b : nat) (lex : (a < b)%nat), representable_X. *)
-(* Proof. *)
-(*   intros a b lex. refine (Build_representable_X _ (param_and_index_in_graph a b lex) (param_and_index_has a b lex) (param_and_index_monotone a b lex)). *)
-(* Defined. *)
+Definition param_and_index_representable : forall  (a b : nat) (lex : (a < b)%nat), representable_X.
+Proof.
+  intros a b lex. refine (Build_representable_X _ (param_and_index_in_graph a b lex) (param_and_index_has a b lex) (param_and_index_monotone a b lex)).
+Defined.
 
-(* (* Code for foo *) *)
-(* Definition param_and_indexCode := *)
-(*   PARAM nat (fun a => PARAM nat (fun b => INDEX (le_representable a b) (fun pf => RES (param_and_index_representable a b pf) ) )). *)
+(* Code for foo *)
+Definition param_and_indexCode :=
+  PARAM nat (fun a => PARAM nat (fun b => INDEX (le_representable a b) (fun pf => RES (param_and_index_representable a b pf) ) )).
 
-(* Definition paramAndIndexDescr : constructor_description. *)
-(* Proof. *)
-(*   refine (Build_constructor_description  _alloc_make_Coq_Init_Datatypes_list_cons param_and_indexCode _). *)
-(*   simpl. intros (a&b&pf&_). simpl. exact (foo a b pf). *)
-(* Defined. *)
+Definition paramAndIndexDescr : constructor_description.
+Proof.
+  refine (Build_constructor_description  _alloc_make_Coq_Init_Datatypes_list_cons param_and_indexCode _).
+  simpl. intros (a&b&pf&_). simpl. exact (foo a b pf).
+Defined.
 
-(* (** 4.4 Dependent arguments - positive_nat_list *)
+(** 4.4 Dependent arguments - positive_nat_list *)
 
 (*  Definition alloc_make_positive_nat_list_cons_spec : ident * funspec := *)
 (* DECLARE _alloc_make_Coq_Init_Datatypes_list_cons *)
@@ -469,35 +413,37 @@ DECLARE _alloc_make_Coq_Init_Datatypes_list_cons
 (*          ) *)
 (*      RETURN  (rep_type_val g' p') *)
 (*      SEP (full_gc g' t_info' roots outlier ti sh). *)
-(*  *) *)
+(*  *)
 
-(* Inductive positive_nat_list : Type := *)
-(* | pnil : positive_nat_list *)
-(* | pcons : forall (x : nat), (0 < x)%nat -> positive_nat_list -> positive_nat_list. *)
+Inductive positive_nat_list : Type :=
+| pnil : positive_nat_list
+| pcons : forall (x : nat), (0 < x)%nat -> positive_nat_list -> positive_nat_list.
 
-(* Variable positive_nat_list_in_graph : graph -> positive_nat_list -> rep_type ->  Prop. *)
+Variable positive_nat_list_in_graph : graph -> positive_nat_list -> rep_type ->  Prop.
 
-(* Variable positive_nat_list_has: forall (g : graph) (n : positive_nat_list) (v : VType), *)
-(*   positive_nat_list_in_graph g n (repNode v) -> graph_has_v g v. *)
+Variable positive_nat_list_has: forall (g : graph) (n : positive_nat_list) (v : VType),
+  positive_nat_list_in_graph g n (repNode v) -> graph_has_v g v.
 
-(* Variable positive_nat_list_c: *)
-(*  forall (g : graph) (to : nat) (lb : raw_vertex_block) (e : list (EType * (VType * VType))) *)
-(*    (n : positive_nat_list) (p : rep_type), *)
-(*  add_node_compatible g (new_copied_v g to) e -> *)
-(*  graph_has_gen g to -> *)
-(*  positive_nat_list_in_graph g n p -> positive_nat_list_in_graph (add_node g to lb e) n p. *)
+Variable positive_nat_list_c:
+ forall (g : graph) (to : nat) (lb : raw_vertex_block) (e : list (EType * (VType * VType)))
+   (n : positive_nat_list) (p : rep_type),
+ add_node_compatible g (new_copied_v g to) e ->
+ graph_has_gen g to ->
+ positive_nat_list_in_graph g n p -> positive_nat_list_in_graph (add_node g to lb e) n p.
 
-(* Definition positive_nat_list_representable : representable_X. *)
-(* refine (Build_representable_X _ positive_nat_list_in_graph positive_nat_list_has positive_nat_list_c). *)
-(* Defined. *)
+Definition positive_nat_list_representable : representable_X.
+refine (Build_representable_X _ positive_nat_list_in_graph positive_nat_list_has positive_nat_list_c).
+Defined.
 
-(* (* Code *) *)
-(* Definition positve_nat_listCode := *)
-(*   DEPARG nat_representable (fun x => ARG (le_representable 0 x) (ARG positive_nat_list_representable (RES positive_nat_list_representable))). *)
+(* Code *)
+Definition positve_nat_listCode :=
+  DEPARG nat_representable (fun x => ARG (le_representable 0 x) (ARG positive_nat_list_representable (RES positive_nat_list_representable))).
 
-(* (* Constructor description *) *)
-(* Definition posNatListDescr : constructor_description. *)
-(* Proof. *)
-(*   refine (Build_constructor_description  _alloc_make_Coq_Init_Datatypes_list_cons positve_nat_listCode _). *)
-(*   simpl. intros (a&b&pf&_). exact (pcons a b pf). *)
-(* Defined. *)
+(* Constructor description *)
+Definition posNatListDescr : constructor_description.
+Proof.
+  refine (Build_constructor_description  _alloc_make_Coq_Init_Datatypes_list_cons positve_nat_listCode _).
+  simpl. intros (a&b&pf&_). exact (pcons a b pf).
+Defined.
+
+*)
