examples/uint63nat/Verif_prog.v
@@ -1,0 +1,114 @@
+Require Import VeriFFI.examples.uint63nat.prog.
+
+Require Import ZArith.
+Require Import Psatz.
+
+Require Import VeriFFI.verification.specs_general.
+
+Require Import VeriFFI.generator.all.
+
+Obligation Tactic := gen.
+MetaCoq Run (gen_for nat).
+MetaCoq Run (gen_for bool).
+
+MetaCoq Run (desc_gen S).
+
+Require Import VST.floyd.proofauto.
+Require Import VeriFFI.examples.uint63nat.glue.
+Require Import VeriFFI.library.meta.
+
+
+Require Import VST.floyd.proofauto.
+Require Import CertiGraph.CertiGC.GCGraph.
+
+From VeriFFI Require Import library.base_representation.
+From VeriFFI Require Import library.meta.
+From VeriFFI Require Import verification.graph_add.
+From VeriFFI Require Import verification.specs_library.
+
+Definition alloc_make_Coq_Init_Datatypes_nat_S_spec : ident * funspec :=
+  DECLARE _alloc_make_Coq_Init_Datatypes_nat_S
+          (alloc_make_spec_general (@desc _ S _) 1).
+
+Instance CompSpecs : compspecs. make_compspecs prog. Defined.
+Definition Vprog : varspecs. mk_varspecs prog. Defined.
+Definition Gprog := [alloc_make_Coq_Init_Datatypes_nat_S_spec].
+
+Lemma intro_prop_through_close_precondition :
+  forall {Espec : OracleKind} Delta (p1 : Prop) f ps LS sf c post,
+  (p1 -> semax Delta (sepcon (close_precondition f ((PROPx ps LS))) sf) c post) ->
+  semax Delta (sepcon (close_precondition f (PROPx (p1 :: ps) LS)) sf) c post.
+Proof.
+  intros.
+  unfold close_precondition in *.
+  simpl in *.
+  eapply semax_pre with (andp (prop p1)
+  (fun rho : environ =>
+        ((EX vals : list val,
+          !! (map (Map.get (te_of rho)) f = map Some vals /\
+              Forall (fun v : val => v <> Vundef) vals) &&
+          PROPx ps LS (ge_of rho, vals))
+            * sf rho)%logic)).
+  2: apply semax_extract_prop; auto.
+  clear H.
+  intro rho.
+  simpl.
+  apply andp_left2.
+  Intro vals.
+  Exists vals.
+  unfold PROPx.
+  simpl.
+  normalize.
+  apply andp_right; auto.
+  apply prop_right; auto.
+Qed.
+
+(* Trying to rewrite with something like: *)
+(* Lemma aux : forall P ps, (A' xs' ps' -> P ps') -> (A xs ps -> P ps) *)
+Lemma combined_sigT_in_arg :
+  forall (A : Type) (P : A -> Type) (T : forall (p : {x : A & P x}), Type),
+     (forall (a1 : A) (a2: P a1), T (a1; a2)) -> (forall (p : {x : A & P x}), T p).
+Proof. intros A P T f p. destruct p. apply f. Qed.
+
+Lemma separate_sigT_in_arg :
+  forall (A : Type) (P : A -> Type) (T : forall (p : {x : A & P x}), Type),
+      (forall (p : {x : A & P x}), T p) -> (forall (a1 : A) (a2: P a1), T (a1; a2)).
+Proof. auto. Qed.
+
+
+Lemma body_alloc_make_Coq_Init_Datatypes_nat_S :
+  semax_body Vprog Gprog
+             f_alloc_make_Coq_Init_Datatypes_nat_S
+             alloc_make_Coq_Init_Datatypes_nat_S_spec.
+Proof.
+  unfold alloc_make_Coq_Init_Datatypes_nat_S_spec.
+  unfold alloc_make_spec_general.
+  start_function1.
+  hnf in xs.
+  repeat (simple apply intro_prop_through_close_precondition; intro).
+  pattern xs.
+
+  (* apply combined_sigT_in_arg. *)
+  (* pattern H. *)
+
+  (* destruct xs. *)
+  (* hnf in xs. *)
+  (* pattern ps. *)
+  (* destruct xs. *)
+  (* (* write a lemma and rewrite *) *)
+  (* destruct ps. *)
+  (* contradiction H0. *)
+  (* destruct a. *)
+
+  (* unfold in_graphs in H0. *)
+  (* destruct H0. *)
+  (* subst. *)
+
+
+  (* erewrite compute_close_precondition_eq. *)
+  (* 2 : { reflexivity.} *)
+  (* 2 : { simpl. reflexivity.} *)
+  (*   Print start_function2. *)
+  (*   start_function2. *)
+  (*   start_function. *)
+Abort.
