examples/uint63nat/model.v
@@ -1,0 +1,121 @@
+Require Import ZArith.
+Require Import Psatz.
+Require Import String.
+Open Scope string.
+
+Require Import VeriFFI.library.modelled.
+Require Import VeriFFI.library.isomorphism.
+Require Import VeriFFI.library.meta.
+
+Require Import VeriFFI.generator.all.
+Obligation Tactic := gen.
+MetaCoq Run (gen_for nat).
+MetaCoq Run (desc_gen S).
+
+Print S_desc.
+
+Require Import VeriFFI.examples.uint63nat.prog.
+
+Module FM <: UInt63.
+  Definition t := {z : nat | z < 2^63}.
+  Definition from_nat (z : nat) : t.
+    exists (Nat.modulo z (2^63)).
+    apply Nat.mod_upper_bound.
+    apply Nat.pow_nonzero.
+    auto.
+  Defined.
+
+  Definition to_nat (z : t) : nat := proj1_sig z.
+
+  Lemma mod63_ok:
+    forall z, (z mod (2^63) < 2^63)%nat.
+  Proof. intro. apply Nat.mod_upper_bound, Nat.pow_nonzero. auto. Qed.
+
+  Definition add (x y: t) : t :=
+  let '(exist xz x_pf) := x in
+  let '(exist yz y_pf) := y in
+  let z := ((xz + yz) mod (2^63))%nat in
+  exist _ z (mod63_ok _).
+
+  Definition mul (x y: t) : t :=
+  let '(exist xz x_pf) := x in
+  let '(exist yz y_pf) := y in
+  let z := ((xz * yz) mod (2^63))%nat in
+  exist _ z (mod63_ok _).
+End FM.
+
+Module UInt63_Proofs.
+  Axiom Isomorphism_t : Isomorphism C.t FM.t.
+
+  Definition from_nat_ep : extern_properties :=
+    {| type_desc :=
+        @TRANSPARENT nat Rep_nat
+           (Some (fun n => @OPAQUE _ _ Isomorphism_t None))
+     ; prim_fn := C.from_nat
+     ; model_fn := FM.from_nat
+     ; c_name := "int63_from_nat"
+     |}.
+
+  Definition to_nat_ep : extern_properties :=
+    {| type_desc :=
+        @OPAQUE _ _ Isomorphism_t
+           (Some (fun n => @TRANSPARENT nat Rep_nat None))
+     ; prim_fn := C.to_nat
+     ; model_fn := FM.to_nat
+     ; c_name := "int63_to_nat"
+     |}.
+
+  Definition add_ep : extern_properties :=
+    {| type_desc :=
+          @OPAQUE _ _ Isomorphism_t
+            (Some (fun i =>
+              @OPAQUE _ _ Isomorphism_t
+                (Some (fun i => @OPAQUE _ _ Isomorphism_t None))))
+     ; prim_fn := C.add
+     ; model_fn := FM.add
+     ; c_name := "int63_add"
+     |}.
+
+  Definition mul_ep : extern_properties :=
+    {| type_desc :=
+          @OPAQUE _ _ Isomorphism_t
+            (Some (fun i =>
+              @OPAQUE _ _ Isomorphism_t
+                (Some (fun i => @OPAQUE _ _ Isomorphism_t None))))
+     ; prim_fn := C.mul
+     ; model_fn := FM.mul
+     ; c_name := "int63_mul"
+     |}.
+
+  Axiom from_nat_properties : model_spec from_nat_ep.
+  Axiom to_nat_properties : model_spec to_nat_ep.
+  Axiom add_properties : model_spec add_ep.
+  Axiom mul_properties : model_spec mul_ep.
+
+  Eval cbn in model_spec from_nat_ep.
+  Eval cbn in model_spec to_nat_ep.
+  Eval cbn in model_spec add_ep.
+
+  Lemma add_assoc : forall (x y z : nat),
+    C.to_nat (C.add (C.from_nat x) (C.add (C.from_nat y) (C.from_nat z))) =
+    C.to_nat (C.add (C.add (C.from_nat x) (C.from_nat y)) (C.from_nat z)).
+  Proof.
+    Check pair.
+    intros x y z.
+    props from_nat_properties.
+    props to_nat_properties.
+    props add_properties.
+    repeat eq_refl_match.
+    rewrite !from_to, !to_from.
+    unfold FM.add, FM.from_nat, FM.to_nat.
+    (* the rest is just a proof about the functional model *)
+    unfold proj1_sig.
+    rewrite <- !(Nat.add_mod y z).
+    rewrite <- !(Nat.add_mod x y).
+    rewrite <- !(Nat.add_mod).
+    f_equal.
+    apply Nat.add_assoc.
+    all: apply Nat.pow_nonzero; auto.
+  Qed.
+
+End UInt63_Proofs.
